src/Lean/Elab/Tactic/BVDecide/Frontend/BVDecide/ReifiedLemmas.lean
@@ -18,52 +18,55 @@ open Lean.Meta
 
 /--
 This function adds the two lemmas:
-- `boolExpr = true → atomExpr = 1#1`
-- `boolExpr = false → atomExpr = 0#1`
-It assumes that `boolExpr` and `atomExpr` are the expressions corresponding to `bool` and `atom`.
-Furthermore it assumes that `atomExpr` is of the form `BitVec.ofBool boolExpr`.
+- `discrExpr = true → atomExpr = lhsExpr`
+- `discrExpr = false → atomExpr = rhsExpr`
+It assumes that `discrExpr`, `lhsExpr` and `rhsExpr` are the expressions corresponding to `discr`,
+`lhs` and `rhs`. Furthermore it assumes that `atomExpr` is of the form
+`if discrExpr = true then lhsExpr else rhsExpr`.
 -/
-def addOfBoolLemmas (bool : ReifiedBVLogical) (atom : ReifiedBVExpr) (boolExpr atomExpr : Expr) :
-    LemmaM Unit := do
-  let some ofBoolTrueLemma ← mkOfBoolTrueLemma bool atom boolExpr atomExpr | return ()
-  LemmaM.addLemma ofBoolTrueLemma
-  let some ofBoolFalseLemma ← mkOfBoolFalseLemma bool atom boolExpr atomExpr | return ()
-  LemmaM.addLemma ofBoolFalseLemma
+def addIfLemmas (discr : ReifiedBVLogical) (atom lhs rhs : ReifiedBVExpr)
+    (discrExpr atomExpr lhsExpr rhsExpr : Expr) : LemmaM Unit := do
+  let some trueLemma ← mkIfTrueLemma discr atom lhs rhs discrExpr atomExpr lhsExpr rhsExpr | return ()
+  LemmaM.addLemma trueLemma
+  let some falseLemma ← mkIfFalseLemma discr atom lhs rhs discrExpr atomExpr lhsExpr rhsExpr | return ()
+  LemmaM.addLemma falseLemma
 where
-  mkOfBoolTrueLemma (bool : ReifiedBVLogical) (atom : ReifiedBVExpr) (boolExpr atomExpr : Expr) :
-      M (Option SatAtBVLogical) := mkOfBoolLemma bool atom boolExpr atomExpr true 1#1
+  mkIfTrueLemma (discr : ReifiedBVLogical) (atom lhs rhs : ReifiedBVExpr)
+      (discrExpr atomExpr lhsExpr rhsExpr : Expr) : M (Option SatAtBVLogical) :=
+    mkIfLemma true discr atom lhs rhs discrExpr atomExpr lhsExpr rhsExpr
 
-  mkOfBoolFalseLemma (bool : ReifiedBVLogical) (atom : ReifiedBVExpr) (boolExpr atomExpr : Expr) :
-      M (Option SatAtBVLogical) := mkOfBoolLemma bool atom boolExpr atomExpr false 0#1
+  mkIfFalseLemma (discr : ReifiedBVLogical) (atom lhs rhs : ReifiedBVExpr)
+      (discrExpr atomExpr lhsExpr rhsExpr : Expr) : M (Option SatAtBVLogical) :=
+    mkIfLemma false discr atom lhs rhs discrExpr atomExpr lhsExpr rhsExpr
 
-  mkOfBoolLemma (bool : ReifiedBVLogical) (atom : ReifiedBVExpr) (boolExpr atomExpr : Expr)
-     (boolVal : Bool) (resVal : BitVec 1) : M (Option SatAtBVLogical) := do
+  mkIfLemma (discrVal : Bool) (discr : ReifiedBVLogical) (atom lhs rhs : ReifiedBVExpr)
+      (discrExpr atomExpr lhsExpr rhsExpr : Expr) : M (Option SatAtBVLogical) := do
+    let resExpr := if discrVal then lhsExpr else rhsExpr
+    let resValExpr := if discrVal then lhs else rhs
     let lemmaName :=
-      match boolVal with
-      | .true => ``Std.Tactic.BVDecide.Reflect.BitVec.ofBool_true
-      | .false => ``Std.Tactic.BVDecide.Reflect.BitVec.ofBool_false
+      if discrVal then
+        ``Std.Tactic.BVDecide.Reflect.BitVec.if_true
+      else
+        ``Std.Tactic.BVDecide.Reflect.BitVec.if_false
+    let discrValExpr := toExpr discrVal
+    let discrVal ← ReifiedBVLogical.mkBoolConst discrVal
 
-    let boolValExpr := toExpr boolVal
-    let boolVal ← ReifiedBVLogical.mkBoolConst boolVal
-    let resExpr := toExpr resVal
-    let resValExpr ← ReifiedBVExpr.mkBVConst resVal
+    let eqDiscrExpr ← mkAppM ``BEq.beq #[discrExpr, discrValExpr]
+    let eqDiscr ← ReifiedBVLogical.mkGate discr discrVal discrExpr discrValExpr .beq
 
-    let eqBoolExpr ← mkAppM ``BEq.beq #[boolExpr, boolValExpr]
-    let eqBool ← ReifiedBVLogical.mkGate bool boolVal boolExpr boolValExpr .beq
-
-    let eqBVExpr ← mkAppM ``BEq.beq #[mkApp (mkConst ``BitVec.ofBool) boolExpr, resExpr]
+    let eqBVExpr ← mkAppM ``BEq.beq #[atomExpr, resExpr]
     let some eqBVPred ← ReifiedBVPred.mkBinPred atom resValExpr atomExpr resExpr .eq | return none
     let eqBV ← ReifiedBVLogical.ofPred eqBVPred
 
     let trueExpr := mkConst ``Bool.true
-    let impExpr ← mkArrow (← mkEq eqBoolExpr trueExpr) (← mkEq eqBVExpr trueExpr)
+    let impExpr ← mkArrow (← mkEq eqDiscrExpr trueExpr) (← mkEq eqBVExpr trueExpr)
     let decideImpExpr ← mkAppOptM ``Decidable.decide #[some impExpr, none]
-    let imp ← ReifiedBVLogical.mkGate eqBool eqBV eqBoolExpr eqBVExpr .imp
+    let imp ← ReifiedBVLogical.mkGate eqDiscr eqBV eqDiscrExpr eqBVExpr .imp
 
     let proof := do
       let evalExpr ← ReifiedBVLogical.mkEvalExpr imp.expr
       let congrProof ← imp.evalsAtAtoms
-      let lemmaProof := mkApp (mkConst lemmaName) boolExpr
+      let lemmaProof := mkApp4 (mkConst lemmaName) (toExpr lhs.width) discrExpr lhsExpr rhsExpr
       return mkApp4
         (mkConst ``Std.Tactic.BVDecide.Reflect.Bool.lemma_congr)
         decideImpExpr
