src/Std/Tactic/BVDecide/Bitblast/BVExpr/Circuit/Impl/Expr.lean
@@ -21,7 +21,6 @@ import Std.Tactic.BVDecide.Bitblast.BVExpr.Circuit.Impl.Operations.SignExtend
 import Std.Tactic.BVDecide.Bitblast.BVExpr.Circuit.Impl.Operations.Mul
 import Std.Tactic.BVDecide.Bitblast.BVExpr.Circuit.Impl.Operations.Udiv
 import Std.Tactic.BVDecide.Bitblast.BVExpr.Circuit.Impl.Operations.Umod
-import Std.Tactic.BVDecide.Bitblast.BVExpr.Circuit.Impl.Operations.Sdiv
 
 /-!
 This module contains the implementation of a bitblaster for `BitVec` expressions (`BVExpr`).
@@ -115,13 +114,6 @@ where
         let res := bitblast.blastUmod aig ⟨lhs, rhs⟩
         have := by
           apply AIG.LawfulVecOperator.le_size_of_le_aig_size (f := bitblast.blastUmod)
-          dsimp only at hlaig hraig
-          omega
-        ⟨res, this⟩
-      | .sdiv =>
-        let res := bitblast.blastSdiv aig ⟨lhs, rhs⟩
-        have := by
-          apply AIG.LawfulVecOperator.le_size_of_le_aig_size (f := bitblast.blastSdiv)
           dsimp only at hlaig hraig
           omega
         ⟨res, this⟩
@@ -235,7 +227,7 @@ theorem bitblast.go_decl_eq (aig : AIG BVBit) (expr : BVExpr w) :
     rw [AIG.LawfulVecOperator.decl_eq (f := blastConst)]
   | bin lhs op rhs lih rih =>
     match op with
-    | .and | .or | .xor | .add | .mul | .udiv | .umod | .sdiv =>
+    | .and | .or | .xor | .add | .mul | .udiv | .umod =>
       dsimp only [go]
       have := (bitblast.go aig lhs).property
       have := (go (go aig lhs).1.aig rhs).property
